code/experimental/aes/Hacl.Impl.Aes.CoreNI.fst
@@ -28,9 +28,9 @@ inline_for_extraction
 val copy_state:
     st: state
   -> ost: state ->
-  ST unit
+  Stack unit
   (requires (fun h -> live h st /\ live h ost))
-  (ensures (fun h0 _ h1 -> modifies (loc st) h0 h1))
+  (ensures (fun h0 _ h1 -> modifies1 st h0 h1))
 
 let copy_state st ost =
   st.(size 0) <- ost.(size 0);
@@ -43,9 +43,9 @@ inline_for_extraction
 val load_block0:
     st: state
   -> b: lbuffer uint8 16ul ->
-  ST unit
+  Stack unit
   (requires (fun h -> live h st /\ live h b))
-  (ensures (fun h0 _ h1 -> modifies (loc st) h0 h1))
+  (ensures  (fun h0 _ h1 -> modifies1 st h0 h1))
 
 let load_block0 st b = st.(size 0) <- vec128_load_le b
 
@@ -54,9 +54,9 @@ inline_for_extraction
 val load_key1:
     k: key1
   -> b: lbuffer uint8 16ul ->
-  ST unit
+  Stack unit
   (requires (fun h -> live h k /\ live h b))
-  (ensures (fun h0 _ h1 -> modifies (loc k) h0 h1))
+  (ensures (fun h0 _ h1 -> modifies1 k h0 h1))
 
 let load_key1 k b = k.(size 0) <- vec128_load_le b
 
@@ -65,9 +65,9 @@ inline_for_extraction
 val load_nonce:
     n: nonce
   -> b: lbuffer uint8 12ul ->
-  ST unit
+  Stack unit
   (requires (fun h -> live h n /\ live h b))
-  (ensures (fun h0 _ h1 -> modifies (loc n) h0 h1))
+  (ensures (fun h0 _ h1 -> modifies1 n h0 h1))
 
 let load_nonce n b =
   push_frame();
@@ -82,9 +82,9 @@ val load_state:
     st: state
   -> nonce: nonce
   -> counter: size_t ->
-  ST unit
+  Stack unit
   (requires (fun h -> live h st /\ live h nonce))
-  (ensures (fun h0 _ h1 -> modifies (loc st) h0 h1))
+  (ensures (fun h0 _ h1 -> modifies1 st h0 h1))
 
 let load_state st nonce counter =
   let counter = secret counter in
@@ -102,9 +102,9 @@ inline_for_extraction
 val store_block0:
     out: lbuffer uint8 16ul
   -> st: state ->
-  ST unit
+  Stack unit
   (requires (fun h -> live h st /\ live h out))
-  (ensures (fun h0 _ h1 -> modifies (loc out) h0 h1))
+  (ensures (fun h0 _ h1 -> modifies1 out h0 h1))
 
 let store_block0 out st =
   vec128_store_le out st.(size 0)
@@ -114,9 +114,9 @@ inline_for_extraction
 val xor_state_key1:
     st: state
   -> key: key1 ->
-  ST unit
+  Stack unit
   (requires (fun h -> live h st /\ live h key))
-  (ensures (fun h0 _ h1 -> live h1 st /\ live h1 key /\ modifies (loc st) h0 h1))
+  (ensures (fun h0 _ h1 -> modifies1 st h0 h1))
 
 let xor_state_key1 st key =
   st.(size 0) <- vec128_xor st.(size 0) key.(size 0);
@@ -130,9 +130,9 @@ val xor_block:
     out: lbuffer uint8 64ul
   -> st: state
   -> b: lbuffer uint8 64ul ->
-  ST unit
+  Stack unit
   (requires (fun h -> live h st /\ live h out /\ live h b))
-  (ensures (fun h0 _ h1 -> modifies (loc out) h0 h1))
+  (ensures (fun h0 _ h1 -> modifies1 out h0 h1))
 
 let xor_block out st inp =
   let v0 = vec128_load_le (sub inp (size 0) (size 16)) in
@@ -153,9 +153,9 @@ inline_for_extraction
 val aes_enc:
     st: state
   -> key: key1 ->
-  ST unit
+  Stack unit
   (requires (fun h -> live h st /\ live h key))
-  (ensures (fun h0 _ h1 -> live h1 st /\ live h1 key /\ modifies (loc st) h0 h1))
+  (ensures (fun h0 _ h1 -> modifies1 st h0 h1))
 
 let aes_enc st key =
   st.(size 0) <- ni_aes_enc st.(size 0) key.(size 0);
@@ -168,9 +168,9 @@ inline_for_extraction
 val aes_enc_last:
     st: state
   -> key: key1 ->
-  ST unit
+  Stack unit
   (requires (fun h -> live h st /\ live h key))
-  (ensures (fun h0 _ h1 -> live h1 st /\ live h1 key /\ modifies (loc st) h0 h1))
+  (ensures (fun h0 _ h1 -> modifies1 st h0 h1))
 
 let aes_enc_last st key =
   st.(size 0) <- ni_aes_enc_last st.(size 0) key.(size 0);
@@ -184,9 +184,9 @@ val aes_keygen_assist:
     ok: key1
   -> ik: key1
   -> rcon: uint8 ->
-  ST unit
+  Stack unit
   (requires (fun h -> live h ok /\ live h ik))
-  (ensures (fun h0 _ h1 -> live h1 ok /\ live h1 ik /\ modifies (loc ok) h0 h1))
+  (ensures (fun h0 _ h1 -> modifies1 ok h0 h1))
 
 let aes_keygen_assist ok ik rcon =
   ok.(size 0) <- ni_aes_keygen_assist ik.(size 0) rcon
@@ -196,9 +196,9 @@ inline_for_extraction
 val key_expansion_step:
     next: key1
   -> prev: key1 ->
-  ST unit
+  Stack unit
   (requires (fun h -> live h prev /\ live h next))
-  (ensures (fun h0 _ h1 -> live h1 prev /\ live h1 next /\ modifies (loc next) h0 h1))
+  (ensures (fun h0 _ h1 -> modifies1 next h0 h1))
 
 let key_expansion_step next prev =
   let n0 = next.(size 0) in
@@ -214,9 +214,9 @@ inline_for_extraction
 val key_expansion_step2:
     next: key1
   -> prev: key1 ->
-  ST unit
+  Stack unit
   (requires (fun h -> live h prev /\ live h next))
-  (ensures (fun h0 _ h1 -> live h1 prev /\ live h1 next /\ modifies (loc next) h0 h1))
+  (ensures (fun h0 _ h1 -> modifies1 next h0 h1))
 
 let key_expansion_step2 next prev =
   next.(size 0) <- vec128_shuffle32 next.(size 0) (vec128_shuffle32_spec (u8 2) (u8 2) (u8 2) (u8 2));
